Assignment 9 Answers:

###1. 	Prove by induction that 1 + 5 + 9 + ... + (4n-3) = n(2n-1)

		n=1
		
		1 = 1(2(1) - 1)
		
		1 = 1(2-1)
		
		1 = 1(1)
		
		1 = 2-1
		
		Base case is true.

		k(2k-1) + (4(k+1)-3) = (k+1)(2(k+1)-1)
		
		(2k^2-k) + (4k+4-3) = (k+1)(2k+2-1)
		
		2k^2-k+4k+1 = (k+1)(2k+1)
		
		2k^2+3k+1 = 2k^2+k+2k+1
		
		Answer: 2k^2+3k+1 = 2k^2+3k+1

###2.	n^3 + 2n = 3m

		n=1

		1 = (1^3 + 2(1)) / 3

		1 = (1 + 2) / 3

		1 = 3 / 3

		1 = 1

		Base case is true

		n^3 = 3m -2n

		(n+1)^3 + 2(n+1) = 3m

		(n+1)(n+1)(n+1) + (2n+2) = 3m

		(n^2+n+n+1)(n+1) + (2n+2) = 3m

		(n^2+2n+1)(n+1) + (2n+2) = 3m

		(n^3+n^2+2n^2+2n+n+1) + (2n+2) = 3m

		(n^3+3n^2+3n+1) + (2n+2) = 3m

		n^3+3n^2+5n+3 = 3m

		(3m-2n)+3n^2+5n+3 = 3m

		3m+3n^2+3n+3 = 3m

		3(m+n^2+n+1) = 3m

		Answer: 3m = 3m

###3.	


